otbn_model/print.dfy
@@ -1,12 +1,12 @@
 // include "../gen/mont_loop.dfy"
 include "gen/modexp_var.dfy"
 include "code/vale.dfy"
+include "gen/mul256.dfy" 
 
 module otbn_printer {
     import opened bv_ops
     import opened vt_ops
     import opened modexp_var
-
 
 method printReg32(r:reg32_t)
 {
@@ -117,7 +117,6 @@ method printFlag(flag:uint2)
         case 1 => print("M");
         case 2 => print("L");
         case 3 => print("Z");
-        case _ => print("ERROR: Invalid flag.");
 }
 
 method printAccShift(shift:int)
@@ -325,6 +324,28 @@ function method procName(proc_name:seq<char>, suffix:seq<char>, asm:AsmTarget, p
 method PrintDemo(asm:AsmTarget, platform:PlatformTarget)
 {
     printProc("modexp_var", va_code_modexp_var());
+}
+
+method ExecuteDemo()
+{
+    // var state: state;
+    // va_code_mul256_w30xw2
+    // datatype state = state(
+    //     gprs: gprs_t, // 32-bit registers
+    //     wdrs: wdrs_t, // 256-bit registers
+
+    //     wmod: uint256,
+    //     wrnd: uint256,
+    //     wacc: uint256,
+
+    //     fgroups: fgroups_t,
+
+    //     xmem: xmem_t,
+    //     wmem: wmem_t,
+
+    //     ok: bool)
+
+    // va_code_modexp_var()
 }
 
 method Main()
